CoqOfRust/examples/default/examples/ink_contracts/Simulations/erc20.v
@@ -60,8 +60,8 @@ Definition transfer_from_to
     (from : erc20.AccountId.t)
     (to : erc20.AccountId.t)
     (value : ltac:(erc20.Balance)) :
-    MS? erc20.Erc20.t ltac:(erc20.Result unit) :=
-  letS? storage := readS? in
+    MS? (erc20.Erc20.t * M.Logs) ltac:(erc20.Result unit) :=
+  letS? '(storage, logs) := readS? in
   let from_balance := balance_of_impl storage from in
   if from_balance <u128 value then
     returnS? (result.Result.Err erc20.Error.InsufficientBalance)
@@ -71,16 +71,23 @@ Definition transfer_from_to
       storage <| erc20.Erc20.balances :=
         Lib.Mapping.insert from new_from_balance
           storage.(erc20.Erc20.balances)
-      |>
+      |>,
+      logs
     ) in
-    letS? storage := readS? in
+    letS? '(storage, logs) := readS? in
     let to_balance := balance_of_impl storage to in
     letS? new_to_balance := return?toS? (BinOp.Error.add to_balance value) in
+    let event := {|
+      erc20.Transfer.from := option.Option.Some from;
+      erc20.Transfer.to := option.Option.Some to;
+      erc20.Transfer.value := value
+    |} in
     letS? _ := writeS? (
       storage <| erc20.Erc20.balances :=
         Lib.Mapping.insert to new_to_balance
           storage.(erc20.Erc20.balances)
-      |>
+      |>,
+      existS _ event :: logs
     ) in
     returnS? (result.Result.Ok tt).
 
@@ -88,21 +95,27 @@ Definition transfer
     (env : erc20.Env.t)
     (to : erc20.AccountId.t)
     (value : ltac:(erc20.Balance)) :
-    MS? erc20.Erc20.t ltac:(erc20.Result unit) :=
+    MS? (erc20.Erc20.t * M.Logs) ltac:(erc20.Result unit) :=
   transfer_from_to (Env.caller env) to value.
 
 Definition approve
     (env : erc20.Env.t)
     (spender : erc20.AccountId.t)
     (value : ltac:(erc20.Balance)) :
-    MS? erc20.Erc20.t ltac:(erc20.Result unit) :=
+    MS? (erc20.Erc20.t * M.Logs) ltac:(erc20.Result unit) :=
   let owner := Env.caller env in
-  letS? storage := readS? in
+  letS? '(storage, logs) := readS? in
+  let event := {|
+    erc20.Approval.owner := (erc20.env env).(ink_contracts.erc20.Env.caller);
+    erc20.Approval.spender := spender;
+    erc20.Approval.value := value
+  |} in
   letS? _ := writeS? (
     storage <| erc20.Erc20.allowances :=
       Lib.Mapping.insert (owner, spender) value
         storage.(erc20.Erc20.allowances)
-    |>
+    |>,
+    existS _ event :: logs
   ) in
   returnS? (result.Result.Ok tt).
 
@@ -111,9 +124,9 @@ Definition transfer_from
     (from : erc20.AccountId.t)
     (to : erc20.AccountId.t)
     (value : ltac:(erc20.Balance)) :
-    MS? erc20.Erc20.t ltac:(erc20.Result unit) :=
+    MS? (erc20.Erc20.t * M.Logs) ltac:(erc20.Result unit) :=
   let caller := Env.caller env in
-  letS? storage := readS? in
+  letS? '(storage, logs) := readS? in
   let allowance := allowance_impl storage from caller in
   if allowance <u128 value then
     returnS? (result.Result.Err erc20.Error.InsufficientAllowance)
@@ -123,12 +136,13 @@ Definition transfer_from
     | result.Result.Err _ => returnS? (result_from_to)
     | result.Result.Ok _ =>
       let new_allowance := BinOp.Optimistic.sub allowance value in
-      letS? storage := readS? in
+      letS? '(storage, logs) := readS? in
       letS? _ := writeS? (
         storage <| erc20.Erc20.allowances :=
           Lib.Mapping.insert (from, caller) new_allowance
             storage.(erc20.Erc20.allowances)
-        |>
+        |>,
+        logs
       ) in
       returnS? (result.Result.Ok tt)
     end.
