CoqOfRust/Proofs/M.v
@@ -1,4 +1,5 @@
 Require Import CoqOfRust.M.
+Require CoqOfRust.Simulations.M.
 
 Module State.
   Class Trait (State Address : Set) : Type := {
@@ -38,53 +39,71 @@ Module Run.
   Inductive t `{State.Trait} {Env A : Set} (env : Env)
       (* Be aware of the order of parameters: the result and final state are at
          the beginning. *)
-      (result : A) (state' : State) :
-      LowM A -> State -> Prop :=
+      (result : A) (state' : State) (logs' : M.Logs) :
+      LowM A -> State -> M.Logs -> Prop :=
   | Pure :
-    t env result state' (LowM.Pure result) state'
-  | CallPrimitiveStateAllocNone {B : Set} (state : State) (v : B)
+    t env result state' logs' (LowM.Pure result) state' logs'
+  | CallPrimitiveStateAllocNone {B : Set}
+      (state : State) (logs : M.Logs) (v : B)
       (k : Ref B -> LowM A) :
-    t env result state' (k (Ref.Imm v)) state ->
-    t env result state' (LowM.CallPrimitive (Primitive.StateAlloc v) k)
-      state
+    t env result state' logs' (k (Ref.Imm v)) state logs ->
+    t env result state' logs' (LowM.CallPrimitive (Primitive.StateAlloc v) k)
+      state logs
   | CallPrimitiveStateAllocSome
-      (address : Address) (v : State.get_Set address) (state : State)
+      (address : Address) (v : State.get_Set address)
+      (state : State) (logs : M.Logs)
       (k : Ref (State.get_Set address) -> LowM A) :
     let r :=
       Ref.MutRef (A := State.get_Set address) (B := State.get_Set address)
         address (fun full_v => full_v) (fun v _full_v => v) in
     State.read address state = None ->
     State.alloc_write address state v = Some state' ->
-    t env result state' (k r) state ->
-    t env result state' (LowM.CallPrimitive (Primitive.StateAlloc v) k) state
+    t env result state' logs' (k r) state logs ->
+    t env result state' logs' (LowM.CallPrimitive (Primitive.StateAlloc v) k)
+      state logs
   | CallPrimitiveStateRead
-      (address : Address) (v : State.get_Set address) (state : State)
+      (address : Address) (v : State.get_Set address)
+      (state : State) (logs : M.Logs)
       (k : State.get_Set address -> LowM A) :
     State.read address state = Some v ->
-    t env result state' (k v) state ->
-    t env result state' (LowM.CallPrimitive (Primitive.StateRead address) k)
-      state
+    t env result state' logs' (k v) state logs ->
+    t env result state' logs'
+      (LowM.CallPrimitive (Primitive.StateRead address) k)
+      state logs
   | CallPrimitiveStateWrite
       (address : Address) (v : State.get_Set address)
-      (state state_inter : State) (k : unit -> LowM A) :
+      (state state_inter : State) (logs : M.Logs)
+      (k : unit -> LowM A) :
     State.alloc_write address state v = Some state_inter ->
-    t env result state' (k tt) state_inter ->
-    t env result state' (LowM.CallPrimitive (Primitive.StateWrite address v) k)
-      state
-  | CallPrimitiveEnvRead (state : State) (k : Env -> LowM A) :
-    t env result state' (k env) state ->
-    t env result state' (LowM.CallPrimitive Primitive.EnvRead k) state
-  | Cast {B : Set} (v : B) (k : B -> LowM A) :
-    t env result state' (LowM.Cast v k) state'
-  | Call {B : Set} (state state_inter : State) (e : LowM B) (v : B)
+    t env result state' logs' (k tt) state_inter logs ->
+    t env result state' logs'
+      (LowM.CallPrimitive (Primitive.StateWrite address v) k)
+      state logs
+  | CallPrimitiveEnvRead
+      (state : State) (logs : M.Logs) (k : Env -> LowM A) :
+    t env result state' logs' (k env) state logs ->
+    t env result state' logs' (LowM.CallPrimitive Primitive.EnvRead k)
+      state logs
+  | CallLog {Log : Set}
+      (state : State) (logs : M.Logs) (log : Log) (k : unit -> LowM A) :
+    t env result state' logs' (k tt) state (existS _ log :: logs)%list ->
+    t env result state' logs'
+      (LowM.CallPrimitive (Primitive.Log log) k)
+      state logs
+  | Cast {B : Set} (state : State) (logs : M.Logs) (v : B) (k : B -> LowM A) :
+    t env result state' logs' (k v) state logs ->
+    t env result state' logs' (LowM.Cast v k) state logs
+  | Call {B : Set}
+      (state state_inter : State) (logs logs_inter : M.Logs)
+      (e : LowM B) (v : B)
       (k : B -> LowM A) :
-    t env v state_inter e state ->
-    t env result state' (k v) state_inter ->
-    t env result state' (LowM.Call e k) state.
+    t env v state_inter logs_inter e state logs ->
+    t env result state' logs' (k v) state_inter logs_inter ->
+    t env result state' logs' (LowM.Call e k) state logs.
 End Run.
 
-Notation "{{ env , state | e ⇓ result | state' }}" :=
-  (Run.t env result state' e state).
+Notation "{{ env , state , logs | e ⇓ result | state' , logs' }}" :=
+  (Run.t env result state' logs' e state logs).
 
 (** Simplify the usual case of read of immediate value. *)
 Lemma read_of_imm {A : Set} (v : A) :
@@ -96,33 +115,35 @@ Qed.
 
 Ltac run_symbolic_state_read :=
   match goal with
-  | |- Run.t _ _ _ (LowM.CallPrimitive (Primitive.StateRead ?address) _) _ =>
+  | |- Run.t _ _ _ _ (LowM.CallPrimitive (Primitive.StateRead ?address) _) _ _ =>
     let H := fresh "H" in
-    epose proof (H := Run.CallPrimitiveStateRead _ _ _ address);
+    epose proof (H := Run.CallPrimitiveStateRead _ _ _ _ address);
     eapply H; [reflexivity|];
     clear H
   end.
 
 Ltac run_symbolic_state_write :=
   match goal with
-  | |- Run.t ?env ?result ?state'
+  | |- Run.t ?env ?result ?state' ?logs'
       (LowM.CallPrimitive (Primitive.StateWrite ?address ?value) ?k)
-      ?state =>
+      ?state ?logs =>
     let H := fresh "H" in
     epose proof (H :=
-      Run.CallPrimitiveStateWrite env result state' address value state _ k);
+      Run.CallPrimitiveStateWrite
+        env result state' logs' address value state _ logs k);
     apply H; [reflexivity|];
     clear H
   end.
 
 Ltac run_symbolic_one_step :=
   match goal with
-  | |- Run.t _ _ _ _ _ =>
+  | |- Run.t _ _ _ _ _ _ _ =>
     (* We do not use [Run.Call] and let the user use existing lemma for this
        case. *)
     apply Run.Pure ||
     apply Run.CallPrimitiveStateAllocNone ||
     apply Run.CallPrimitiveEnvRead ||
+    apply Run.CallLog ||
     apply Run.Cast ||
     run_symbolic_state_read ||
     run_symbolic_state_write
